[TM computable to BSM computable] Add reworked proof

theories/StackMachines/Reductions/SBTM_HALT_to_HaltBSM.v
@@ -34,12 +34,8 @@ Section Construction.
     | (ls, a, rs) => [ ls ; [a]%list ; rs ; []%list ]%vector
     end.
 
-    Print proj1_sig.
-    Print sval.
-
-  (* Shift everything back by one*)
+  (* Shift everything back by one *)
   Definition encode_state (q : state M) := (1 + shift + sval (Fin.to_nat q) * c).
-
 
   #[local] Arguments encode_state : simpl never.
   #[local] Notation "! p" := (encode_state p) (at level 1).
@@ -48,21 +44,16 @@ Section Construction.
 
   #[local] Notation JMP i := (POP ZERO i i).
 
-  (* Jump after Program now*)
-  Notation END := (1 + shift + c * (num_states M)).
-  
-  (* THIS needs to be adapted somehow, but how to deal with length? -> Keep length at 2 *)
-  (* Definition box '(q, a) (f : (state M * bool * direction) -> list (bsm_instr 4)) : bsm_instr 4 :=
-    match δ (q, a) with
-    | None => PUSH CURR a :: JMP END :: []
-    | Some t => DUMMY INSTRUCTION :: f t :: []
-    end. *)
+  (* Jump after Program now *)
+  Notation POST_TRUE := (1 + shift + c * (num_states M)).
+  Notation POST_FALSE := (3 + shift + c * (num_states M)).
+  Notation END := (5 + shift + c * (num_states M)).
 
   Definition box '(q, a) (f : (state M * bool * direction) -> bsm_instr 4) : bsm_instr 4 :=
-  match δ (q, a) with
-  | None => JMP END
-  | Some t => f t
-  end.
+    match δ (q, a) with
+    | None => JMP (if a then POST_TRUE else POST_FALSE)
+    | Some t => f t
+    end.
 
   Definition CURR' := CURR. (* to distinguish duplicate operations for subcode_tac *)
 
@@ -90,59 +81,35 @@ Section Construction.
 
   Opaque c.
 
+  Lemma c_spec : c = 13.
+  Proof. easy. Qed.
+
   Fixpoint all_fins (n : nat) : list (Fin.t n) :=
     if n is S n' then Fin.F1 :: map Fin.FS (all_fins n') else nil.
 
+  Definition POST : list (bsm_instr 4) :=
+    PUSH CURR' true ::
+    JMP END ::
+    PUSH CURR' false :: 
+    JMP END :: [].
+
   (* constructed BSM *)
   Definition P : list (bsm_instr 4) :=
-    JMP (!q0) :: flat_map PROG (all_fins (num_states M)).
+    JMP (!q0) :: flat_map PROG (all_fins (num_states M)) ++ POST.
 
-  Lemma P_length : length P = 1 + num_states M * c.
+  Lemma length_flat_map_PROG_M : length (flat_map PROG (all_fins (num_states M))) = num_states M * c.
   Proof.
-    simpl.
-    congr S.
     have := PROG_length.
-    elim: (num_states M) (PROG). (* Works like induction ?*)
-    - done.
-    - intros n IH PROG' H.
-      have ->: S n * c = n * c + c by lia.
-      simpl.
-      rewrite length_app.
-      rewrite flat_map_concat_map.
-      rewrite map_map.
-      rewrite <- flat_map_concat_map.
-      rewrite H.
-      rewrite IH.
-      + done.
-      + lia.
+    elim: (num_states M) (PROG); first done.
+    move=> n IH PROG' H. have ->: S n * c = n * c + c by lia.
+    rewrite /= length_app flat_map_concat_map map_map -flat_map_concat_map H.
+    by rewrite IH; [|lia].
   Qed.
 
-  Lemma P_length' : shift + length P = END.
+  Lemma P_length : length P = 5 + num_states M * c.
   Proof.
-    rewrite P_length.
-    cbn.
-    lia.
+    rewrite /= length_app /= length_flat_map_PROG_M. lia.
   Qed.
-
-  Lemma P_length'' : S (length (flat_map (PROG) (all_fins (num_states M)))) =
-S (c * num_states M).
-  Proof.
-    congr S.
-    have := PROG_length.
-    elim: (num_states M) (PROG).
-    - done.
-    - intros n IH PROG' H.
-      simpl.
-      rewrite length_app.
-      rewrite flat_map_concat_map.
-      rewrite map_map.
-      rewrite <- flat_map_concat_map.
-      rewrite H.
-      rewrite IH.
-      + done.
-      + lia.
-  Qed.
-
 
   Definition Q_step (Q : list (bsm_instr 4)) offset i v : option (bsm_state 4) :=
     match nth_error Q i with
@@ -158,38 +125,23 @@ S (c * num_states M).
 
   Arguments Q_step : simpl never.
 
-  Print sss_step.
-
   (* If Q_Step returns Some, then the step is valid according to sss_step *)
   Lemma Q_step_spec (Q : list (bsm_instr 4)) offset i v j w : 
     Q_step Q offset i v = Some (j, w) ->
     sss_step (bsm_sss (n:=4)) (offset, Q) (i + offset, v) (j, w).
   Proof.
-    unfold Q_step.
-    case E: (nth_error Q i) => [t|].
-    - move: E => /(@nth_error_split (bsm_instr 4)) => - [l] [r] [-> <-].
-      intros Ht.
-      exists offset, l, t, r, v. 
-      split.
-      + done.
-      + split.
-        * congr pair.
-          lia.
-        * move: t Ht => [].
-          -- move=> x p' q' [<-].
-             move Ex: (vec_pos v x) => [|[] ?].
-             ++ auto using bsm_sss.
-             ++ auto using bsm_sss.
-             ++ auto using bsm_sss.
-          -- move=> x b [<-] <-.
-             auto using bsm_sss. 
-    - done.
+    rewrite /Q_step. case E: (nth_error Q i) => [t|]; last done.
+    move: E => /(@nth_error_split (bsm_instr 4)) => - [l] [r] [-> <-].
+    move=> Ht. exists offset, l, t, r, v. split; [|split]; [done|congr pair; lia|].
+    move: t Ht => [].
+    - move=> x p' q' [<-].
+      move Ex: (vec_pos v x) => [|[] ?]; by auto using bsm_sss.
+    - move=> x b [<-] <-. by auto using bsm_sss.
   Qed.
 
   Arguments nth_error : simpl never.
 
-  (* If SBTM does a step, then BSM does the same step encoded
-     k?*)
+  (* If SBTM does a step, then BSM does the same step encoded k?*)
   Lemma PROG_spec_Some q t q' t' : step M (q, t) = Some (q', t') ->
     exists k, (!q, PROG q) // (encode_config (q, t)) -[S k]-> (encode_config (q', t')).
   Proof.
@@ -198,73 +150,78 @@ S (c * num_states M).
     move=> [<- <-]. have ->: !q = 0 + !q by done.
     move: d a ls rs E => [] [] [|[] ls] [|[] rs] E.
     all: eexists; rewrite /PROG /box E.
-
-    1: do ? ((by apply: in_sss_steps_0) || (apply: in_sss_steps_S; [by apply: Q_step_spec|])).
-
-
     all: do ? ((by apply: in_sss_steps_0) || (apply: in_sss_steps_S; [by apply: Q_step_spec|])).
   Qed.
 
-  Lemma PROG_spec_None q t : step M (q, t) = None ->
-    exists v, (!q, PROG q) // (encode_config (q, t)) ->> (shift + length P, v).
+  Lemma PROG_spec_None a q ls rs : step M (q, (ls, a, rs)) = None ->
+    (!q, PROG q) // (encode_config (q, (ls, a, rs))) ->> (if a then POST_TRUE else POST_FALSE, [ls; []%list; rs; []%list]%vector).
   Proof.
-    rewrite P_length'.
-    move: t => [[ls a] rs] /=. rewrite /step.
-    case E: (δ (q, a)) => [[[??]d]|]; first done.
-    move=> _. have ->: !q = 0 + !q by done.
-    move: a E => [] E.
-    all: exists [ ls ; []%list ; rs ; []%list ]%vector.
-    all: eexists; rewrite /PROG /box E.
-    all: do ? ((by apply: in_sss_steps_0) || (apply: in_sss_steps_S; [by apply: Q_step_spec|])).
+    rewrite /step.
+    case E: (δ (q, a)) => [[[??]?]|]; first done.
+    move=> _.
+    rewrite /PROG. eexists _.
+    apply in_sss_steps_S with (st2:= (if a then 1 +! q else 7 +! q, [ls; []%list; rs; []%list]%vector)).
+    { eexists _, [], _, _, _.
+      split; [reflexivity|split; [by rewrite (Nat.add_comm (!q))|]].
+      replace ([ls; []%list; rs; []%list]%vector) with (vec_change ([ls; [a]%list; rs; []%list]%vector) CURR' []) by done.
+      destruct a; by constructor. }
+    apply in_sss_steps_S with (st2:= (if a then POST_TRUE else POST_FALSE, [ls; []%list; rs; []%list]%vector)).
+    { destruct a.
+      - eexists _, [_], _, _, _.
+        split; [reflexivity|split; [by rewrite (Nat.add_comm (!q))|]].
+        rewrite /= E. by constructor.
+      - eexists _, [_; _; _; _; _; _; _], _, _, _.
+        split; [reflexivity|split; [by rewrite (Nat.add_comm (!q))|]].
+        rewrite /= E; by constructor. }
+    by apply: in_sss_steps_0.
   Qed.
-
-  Lemma PROG_spec_None_output q t : step M (q, t) = None ->
-    (!q, PROG q) // (encode_config (q, t)) ->> (shift + length P, encode_tape t).
-  Proof.
-    (* rewrite P_length'.
-    move: t => [[ls a] rs] /=. rewrite /step.
-    case E: (δ (q, a)) => [[[??]d]|]; first done.
-    (* move=> _. have ->: !q = 0 + !q by done. *)
-    intros.
-
-    eexists (1 + _).
-    destruct a.
-    -
-    -
-    unfold PROG.
-
-
-
-
-
-
-
-
-    move: a E => [] E.
-    
-
-
-
-
-
-    (* all: exists [ ls ; []%list ; rs ; []%list ]%vector. *)
-    (* all: eexists; rewrite /PROG /box E.  *)
-    all: do ? ((by apply: in_sss_steps_0) || (apply: in_sss_steps_S; [by apply: Q_step_spec|])). *)
-  Admitted.
 
   Lemma PROG_sc (q : state M) : (!q, PROG q) <sc (shift, P).
   Proof.
-    apply: subcode_cons. rewrite /P /encode_state [1+shift]/=.
-    suff: forall n, (n + sval (Fin.to_nat q) * c, PROG q) <sc
-      (n, flat_map PROG (all_fins (num_states M))) by done.
-    have := PROG_length. move: (num_states M) q (PROG) => ?.
-    elim. { move=> /= *. by eexists [], _. }
-    move=> m q IH PROG' H' n.
-    have := IH (fun q => PROG' (Fin.FS q)) => /(_ ltac:(done) (n+c)).
-    rewrite /= !flat_map_concat_map map_map -!flat_map_concat_map.
-    move=> [l] [r] [{}IH {}IH']. exists (PROG' Fin.F1 ++ l), r. split.
-    - by rewrite IH -app_assoc.
-    - move: (Fin.to_nat q) IH' => [? ?] /=. rewrite length_app H'. lia.
+    apply: subcode_cons.
+    apply: subcode_app_end.
+    suff: forall n, (n + shift + sval (Fin.to_nat q) * c, PROG q) <sc
+      (n + shift, flat_map PROG (all_fins (num_states M))) by apply.
+    move: (num_states M) q (PROG) (PROG_length)=> ?.
+    elim; first by eexists [], _.
+    move=> m q IH PROG' H' n. apply: subcode_trans.
+    - have := (IH (fun q => PROG' (Fin.FS q)) (fun q => H' (Fin.FS q)) (n+c)).
+      congr subcode. congr pair.
+      rewrite /=. move: (Fin.to_nat q) => [] /=. lia.
+    - rewrite /= !flat_map_concat_map map_map -!flat_map_concat_map.
+      exists (PROG' Fin.F1), []. rewrite app_nil_r H'.
+      by split; [|lia].
+  Qed.
+
+  Lemma POST_spec a ls rs:
+    (POST_TRUE, POST) // (if a then POST_TRUE else POST_FALSE, [ls; []%list; rs; []%list]%vector) ->> (END, encode_tape (ls, a, rs)).
+  Proof.
+    exists 2.
+    apply in_sss_steps_S with (st2:= (1 + if a then POST_TRUE else POST_FALSE, [ls; [a]%list; rs; []%list]%vector)).
+    { case: a.
+      - eexists _, [], _, _, _.
+        split; [reflexivity|split;[by rewrite (Nat.add_comm _ (length _))|]].
+        by constructor.
+      - eexists _, [_; _], _, _, _.
+        split; [reflexivity|split;[by rewrite (Nat.add_comm _ (length _))|]].
+        by constructor. }
+    apply in_sss_steps_S with (st2:= (END, [ls; [a]%list; rs; []%list]%vector)).
+    { case: a.
+      - eexists _, [_], _, _, _.
+        split; [reflexivity|split;[by rewrite (Nat.add_comm _ (length _))|]].
+        by constructor.
+      - eexists _, [_; _; _], _, _, _.
+        split; [reflexivity|split;[by rewrite (Nat.add_comm _ (length _))|]].
+        by constructor. }
+    by apply in_sss_steps_0.
+  Qed.
+
+  Lemma POST_sc : (POST_TRUE, POST) <sc (shift, P).
+  Proof.
+    eexists (_ :: _), [].
+    rewrite app_nil_r /=.
+    split; first done.
+    rewrite length_flat_map_PROG_M. lia.
   Qed.
 
   (* Opaque P. *)
@@ -278,67 +235,32 @@ S (c * num_states M).
   Qed.
 
   Lemma simulation_step_None q t : step M (q, t) = None ->
-    exists v, (shift, P) // (encode_config (q, t)) ->> (shift + length P, v).
-  Proof.
-    move=> /PROG_spec_None [v Hv]. exists v.
-    by apply: subcode_sss_compute; [apply: PROG_sc|].
-  Qed.
-
-    Lemma simulation_step_None_output q t : step M (q, t) = None ->
     (shift, P) // (encode_config (q, t)) ->> (shift + length P, encode_tape t).
   Proof.
-    move=> /PROG_spec_None_output Hv.
-
-    assert (H1 := PROG_sc q).
-    assert (H2 := subcode_sss_compute).
-    specialize (H2 _ _ _ _ _ _ _ H1 Hv).
-    apply H2.
+    move: t => [[ls a] rs] /PROG_spec_None.
+    have /subcode_sss_compute := PROG_sc q.
+    move=> /[apply] /sss_compute_trans. apply.
+    apply: subcode_sss_compute; first by apply POST_sc.
+    have ->: shift + length P = END.
+    { rewrite P_length. cbn. lia. }
+    by apply: POST_spec.
   Qed.
-
-  Lemma simulation q t k :
-    steps M k (q, t) = None ->
-    exists v, (shift, P) // (encode_config (q, t)) ->> (shift + length P, v).
-  Proof.
-    elim: k q t; first done.
-    move=> k IH q t. rewrite (steps_plus 1) /=.
-    case E: (step M (q, t)) => [[q' t']|].
-    - move=> /IH [v] Hv. exists v.
-      move: E => /simulation_step_Some [?] /sss_steps_compute /sss_compute_trans.
-      by apply.
-    - by move: E => /simulation_step_None.
-  Qed.
-
 
   Lemma simulation_output q q' t t' k :
     steps M k (q, t) = Some (q', t') ->
     (shift, P) // (encode_config (q, t)) ->> (encode_config (q', t')).
   Proof.
     elim: k q t.
-    + intros.
-      injection H.
-      intros.
-      subst.
-      simpl.
-      unfold sss_compute.
+    - move=> ?? [-> ->].
       exists 0.
-      constructor.
-    +
-    move=> k IH q t. rewrite (steps_plus 1) /=.
-    case E: (step M (q, t)) => [[q'' t'']|].
-    - move=> /IH [v] Hv.
-
-      assert (Y := simulation_step_Some).
-      specialize (Y _ _ _ _ E).
-      destruct Y.
-
-      exists ((S x) + v).
-
-      assert (X := sss_steps_trans).
-      specialize (X _ _ _ _ _ _ _ _ _ H Hv).
-      simpl in X.
-      apply X.
-
-    - by move: E => /simulation_step_None.
+      by constructor.
+    - move=> k IH q t. rewrite (steps_plus 1) /=.
+      case E: (step M (q, t)) => [[q'' t'']|].
+      + move=> /IH [v] Hv.
+        move: E => /simulation_step_Some [k' Hk'].
+        exists ((S k') + v).
+        apply: sss_steps_trans; by eassumption.
+      + by move: E => /simulation_step_None.
   Qed.
 
   Lemma simulation_output'' q q' t t' k :
@@ -346,143 +268,59 @@ S (c * num_states M).
     steps M (S k) (q, t) = None ->
     (shift, P) // (encode_config (q, t)) ->> (shift + length P, encode_tape t').
   Proof.
-    elim: k q t.
-    + intros.
-
-      assert (H2 := simulation_output).
-      specialize (H2 _ _ _ _ _ H).
-      unfold sss_compute in H2.
-      destruct H2 as [k H2].
-
-      assert (X := simulation_step_None_output).
-      specialize (X _ _ H0).
-
-      inversion H.
-      subst.
-      apply X.
-
-    +
-    move=> k IH q t.
-    intros. 
-    replace (S k) with (1 + k) in H by lia.
-    replace (S (S k)) with (1 + (S k)) in H0 by lia.
-    rewrite steps_plus in H.
-    rewrite steps_plus in H0.
-    case E: (step M (q, t)) => [[q'' t'']|].
-    - 
-      
-      simpl in H.
-      rewrite E in H.
-
-      replace (steps M 1 (q, t)) with (step M (q,t)) in H0 by easy.
-      rewrite E in H0.
-
-      simpl in H.
-      simpl in H0.
-
-      replace (SBTM.obind (step M) (steps M k (q'', t''))) with (steps M (S k) (q'', t'')) in H0 by easy.
-      
-      specialize (IH _ _ H H0).
-
-      destruct IH as [k0 IH].
-
-
-      assert (Y := simulation_step_Some).
-      specialize (Y _ _ _ _ E).
-      destruct Y.
-
-      exists ((S x) + k0).
-
-      assert (X := sss_steps_trans).
-      specialize (X _ _ _ _ _ _ _ _ _ H1 IH).
-      apply X.
-
-    - simpl in H.
-      rewrite E in H.
-      simpl in H.
-      inversion H.
+    have ->: S k = k + 1 by lia.
+    rewrite (steps_plus).
+    move=> /[dup] /simulation_output /sss_compute_trans + -> /= H. apply.
+    by apply: simulation_step_None.
   Qed.
 
-
-
-    Lemma simulation' t k :
-    steps M k (q0, t) = None ->
-    exists v, (shift, P) // (shift, encode_tape t) ->> (shift + length P, v).
+  Lemma simulation q t k :
+    steps M k (q, t) = None ->
+    exists v, (shift, P) // (encode_config (q, t)) ->> (shift + length P, v).
   Proof.
-    intros H0.
-    destruct k.
-    - inversion H0.
-    - assert (H1 := simulation).
-      specialize (H1 q0 t (S k) H0).
-      destruct H1 as [v H1].
-      exists v.
-      unfold sss_compute in H1.
-      destruct H1 as [k0 H1].
-      unfold sss_compute.
-      exists (S k0).
-
-      assert (H5 := in_sss_steps_S).
-      specialize (H5 _ _ (bsm_sss (n:= 4)) (shift, P) k0 (shift, encode_tape t) (!q0, encode_tape t) (shift + length P, v)).
-      apply H5.
-      + unfold P.
-        unfold sss_step. 
-        exists shift.
-        exists [].
-        exists (JMP ! q0).
-        exists (flat_map PROG (all_fins (num_states M))).
-        exists (encode_tape t).
-        split.
-        * auto.
-        * split.
-          -- simpl.
-            replace (shift + 0) with shift by lia.
-            reflexivity.
-          -- apply in_bsm_sss_pop_E.
-            unfold encode_tape.
-            destruct t as [p rs].
-            destruct p as [ls a].
-            reflexivity.
-      + apply H1.
+    elim: k q t; first done.
+    move=> k IH q t /[dup] HSk.
+    have ->: S k = k + 1 by lia.
+    rewrite steps_plus.
+    case E: (steps M k (q, t)) => [[q' t']|].
+    - move: E HSk => /simulation_output'' /[apply] ??.
+      eexists. by eassumption.
+    - move=> ?. by apply: IH.
   Qed.
 
+  Lemma sss_step_shift t : sss_step (bsm_sss (n:=4)) (shift, P) (shift, encode_tape t) (encode_config (q0, t)).
+  Proof.
+    eexists _, [], _, _, _.
+    split; [reflexivity|split; [by rewrite Nat.add_comm|]].
+    move: (t) => [[??]?].
+    by constructor.
+  Qed.
 
-      Lemma simulation_output' q' t t' k :
+  Lemma simulation_output' q' t t' k :
     steps M k (q0, t) = Some (q', t') ->
     steps M (S k) (q0, t) = None ->
     (shift, P) // (shift, encode_tape t) ->> (shift + length P, encode_tape t').
   Proof.
-    intros H0 H1.
-
-    assert (H2 := simulation_output'').
-    specialize (H2 q0 q' t t' k H0 H1).
-    unfold sss_compute in H2.
-    destruct H2 as [k0 H2].
-    unfold sss_compute.
-    exists (1 + k0).
-
-    assert (A : (shift, P) // (shift, encode_tape t) -[1]-> encode_config (q0, t)).
-    - apply sss_steps_1.
-      unfold sss_step.
-      unfold P.
-      exists shift.
-      eexists [].
-      eexists (JMP ! q0).
-      eexists (flat_map PROG (all_fins (num_states M))).
-      eexists (encode_tape t).
-      split.
-      +  cbn. reflexivity.
-      + split.
-        * cbn. replace (shift + 0) with shift by lia. reflexivity.
-        * apply in_bsm_sss_pop_E.
-            unfold encode_tape.
-            destruct t.
-            destruct p.
-            reflexivity.
-    - assert (T := sss_steps_trans).
-      specialize (T _ _ _ _ _ _ _ _ _ A H2).
-      apply T.
+    move=> /simulation_output'' /[apply] ?.
+    apply: sss_compute_trans; last by eassumption. 
+    exists 1.
+    apply: in_sss_steps_S; last by apply: in_sss_steps_0.
+    by apply: sss_step_shift.
   Qed.
 
+  Lemma simulation' t k :
+    steps M k (q0, t) = None ->
+    exists v, (shift, P) // (shift, encode_tape t) ->> (shift + length P, v).
+  Proof.
+    elim: k; first done.
+    move=> k IH /[dup] HSk.
+    have ->: S k = k + 1 by lia.
+    rewrite steps_plus.
+    case E: (steps M k (q0, t)) => [[??]|].
+    - move: E HSk => /simulation_output' /[apply] *.
+      eexists. by eassumption.
+    - move=> ?. by apply: IH.
+  Qed.
 
   Lemma inverse_simulation q t n i v :
     (shift, P) // (encode_config (q, t)) -[n]-> (shift + i, v) ->
@@ -490,9 +328,11 @@ S (c * num_states M).
     exists k, steps M k (q, t) = None.
   Proof.
     elim /(Nat.measure_induction _ id) : n q t => - [|n] IH q t.
-    { move=> /sss_steps_0_inv [] /= <- _.
-      rewrite /encode_state P_length'' (ltac:(done) : c = (S (c-1))).
-      have := svalP (Fin.to_nat q). nia. }
+    { move=> /sss_steps_0_inv [] /= <- _ [|].
+      - rewrite /encode_state. lia.
+      - rewrite /encode_state length_app length_flat_map_PROG_M.
+        destruct (Fin.to_nat q).
+        cbn. nia. }
     case E: (step M (q, t)) => [[q' t']|]; last by (move=> _; exists 1).
     move: (E) => /simulation_step_Some [m].
     move=> Hn Hm Hi. have := (IH (n - m) ltac:(lia) q' t' _ Hi).
@@ -506,71 +346,22 @@ S (c * num_states M).
   Qed.
 
   Lemma inverse_simulation' t n i v :
-    (shift, P) // (shift , encode_tape t) -[n]-> (shift + i, v) ->
+    (shift, P) // (shift, encode_tape t) -[n]-> (shift + i, v) ->
     out_code (shift + i) (shift, P) ->
     exists k, steps M k (q0, t) = None.
   Proof.
-    intros H0 H1.
-    induction n.
-    - destruct i.
-      + inversion H1; cbn in H; lia.
-      + inversion H0. lia.
-    - assert (H2 := inverse_simulation).
-      specialize (H2 q0 t n i v).
-      apply H2.
-      + assert (H3 := sss_steps_S_inv').
-        specialize (H3 _ _ (bsm_sss (n:= 4)) (shift, P) (shift, encode_tape t) (shift + i, v) n H0).
-        destruct H3 as [str2 H3].
-        destruct H3 as [H3A H3B].
-        unfold sss_step in H3A.
-        destruct H3A.
-        destruct H.
-        destruct H.
-        destruct H.
-        destruct H.
-        destruct H.
-        destruct H3.
-        injection H.
-        injection H3.
-        intros.
-        assert (H9 : x0 = []).
-        * rewrite H8 in H6. 
-          assert (length x0 = 0) by lia.
-          apply length_zero_iff_nil.
-          apply H9.
-        *
-        rewrite H9 in H7.
-        replace ([] ++ x1 :: x2) with (x1 :: x2) in H7 by auto.
-        unfold P in H7.
-        inversion H7.
-        rewrite <- H11 in H4.
-        inversion H4.
-        -- rewrite <- H13 in H3B. apply H3B.
-        -- unfold encode_tape in H18.
-          destruct t in H18.
-          destruct p0 in H18.
-          simpl in H18.
-          inversion H18.
-        -- unfold encode_tape in H18.
-          destruct t in H18.
-          destruct p0 in H18.
-          simpl in H18.
-          inversion H18.
-      + apply H1.
+    case: n.
+    - move=> /sss_steps_0_inv [] <- _ /=. lia.
+    - move=> n /sss_steps_S_inv' [[q' t']] [].
+      have := @bsm_sss_fun 4.
+      have := sss_step_shift t.
+      move=> /sss_step_fun /[apply] /[apply] <-.
+      by apply: inverse_simulation.
 Qed.
-
-
-    
-      
-
-
-
 
 End Construction.
 
 Require Import Undecidability.Synthetic.Definitions.
-
-Arguments mult _ _ : simpl never.
 
 Theorem reduction :
   SBTM_HALT ⪯ BSM_HALTING.
@@ -579,13 +370,12 @@ Proof.
     existT _ 4 (existT _ 0 (existT _ (@P M q 0) (encode_tape t)))).
   move=> [M [q [[ls a] rs]]]. split.
   - move=> [k] /simulation => /(_ q 0) [v Hv] /=.
-    exists ((1 + c * (num_states M)), v). split => /=.
+    exists ((5 + (num_states M) * c), v). split => /=.
     + rewrite /P.
-      rewrite P_length' in Hv.
+      rewrite P_length in Hv.
       bsm sss POP empty with ZERO (encode_state M 0 q ) (encode_state M 0 q).
     + right.
-      rewrite <- (P_length'' M 0).
-      constructor.
+      rewrite length_app length_flat_map_PROG_M /=. lia.
   - move=> [] [i v] [] [?] H /= ?.
     rewrite /P in H.
     bsm inv POP empty with H ZERO (encode_state M 0 q) (encode_state M 0 q).
