theories/TM/Reductions/HaltTM_1_to_SBTM_HALT.v
@@ -4,7 +4,6 @@ Require Import Undecidability.Shared.Libs.PSL.FiniteTypes.FinTypes.
 
 From Stdlib Require Import PeanoNat Lia.
 
-
 #[local] Unset Implicit Arguments.
 #[local] Unset Strict Implicit.
 
@@ -16,12 +15,69 @@ Set Default Goal Selector "!".
 
 Module SBTM_facts.
 
-  (* remove redundante false symbol *)
-  Definition truncate (l : list bool) : list bool :=
+  (* TODO move almost_eq and almost_eq_tape Lemmas to SBTM_facts *)
+  Lemma almost_eq_elim l1 l2 :
+    almost_eq l1 l2 -> 
+    match l1 with
+    | [] => l2 = repeat false (length l2)
+    | a :: l1' =>
+        match l2 with
+        | [] => l1 = repeat false (length l1)
+        | b :: l2' => a = b /\ almost_eq l1' l2'
+        end
+    end.
+  Proof.
+    elim; first done.
+    move=> [|?] [|?].
+    - reflexivity.
+    - by rewrite repeat_length.
+    - by rewrite /= repeat_length.
+    - by repeat constructor.
+  Qed.
+
+  Lemma almost_eq_false_spec m l :
+    almost_eq (repeat false m) l -> l = repeat false (length l).
+  Proof.
+    elim: m l.
+    - move=> [|??]; first done.
+      move=> /almost_eq_elim /= [-> ->]. by rewrite repeat_length.
+    - move=> m IH [|??]; first done.
+      move=> /almost_eq_elim /= [<-] /IH ?.
+      by congr cons.
+  Qed.
+
+  Lemma almost_eq_trans l1 l2 l3 :
+    almost_eq l1 l2 -> almost_eq l2 l3 -> almost_eq l1 l3.
+  Proof.
+    move=> H. elim: H l3.
+    - move=> > H IH [|??] /almost_eq_elim /=.
+      + move=> [->] E.
+        move: H. rewrite E=> /almost_eq_sym /almost_eq_false_spec ->.
+        by apply: (almost_eq_false (S _) 0).
+      + move=> [<-] ?. constructor. by apply: IH.
+    - move=> > /almost_eq_false_spec ->. by constructor.
+  Qed.
+
+  Lemma almost_eq_tape_refl t :
+    almost_eq_tape t t.
+  Proof.
+    move: t => [[ls a] rs].
+    constructor; by apply: almost_eq_refl.
+  Qed.
+
+  Lemma almost_eq_tape_trans t1 t2 t3 :
+    almost_eq_tape t1 t2 -> almost_eq_tape t2 t3 -> almost_eq_tape t1 t3.
+  Proof.
+    move=> [> ??] H. inversion H. subst.
+    constructor; apply: almost_eq_trans; by eassumption.
+  Qed.
+
+  (* remove redundant false symbols by Alexandra Latys *)
+  Fixpoint truncate (l : list bool) : list bool :=
+    if forallb negb l then [] else
     match l with
-    | [false] => []
-    | [a; false] => if a then [a] else []
-    | _ => l
+    | a :: l' => a :: truncate l'
+    | [] => []
     end.
 
   Definition truncate_tape (t : tape) : tape :=
@@ -31,11 +87,16 @@ Module SBTM_facts.
 
   Lemma almost_eq_truncate l : almost_eq (truncate l) l. 
   Proof.
-    have ? := almost_eq_refl.
-    have ? := almost_eq_false 0 0.
-    have ? := almost_eq_false 0 1.
-    have ? := almost_eq_false 0 2.
-    move: l => [|[] [|[] [|??]]] /=; by do ? constructor.
+    elim: l => [|[|] l IH] /=.
+    - by apply: almost_eq_false 0 0.
+    - by constructor.
+    - case E: (forallb negb l).
+      + suff: l = repeat false (length l).
+        { move=> ->. by apply: almost_eq_false 0 (S (length l)). }
+        apply /Forall_eq_repeat /Forall_forall => a.
+        move: E => /forallb_forall /[apply].
+        by case: a.
+      + by constructor.
   Qed.
 
   Lemma almost_eq_tape_truncate_tape t : almost_eq_tape (truncate_tape t) t.
@@ -43,58 +104,60 @@ Module SBTM_facts.
     move: t => [[ls a] rs]. constructor; by apply: almost_eq_truncate.
   Qed.
 
+    Lemma truncate_repeat_false n : truncate (repeat false n) = [].
+  Proof.
+    elim: n; first done.
+    move=> n IH /=.
+    case E: (forallb negb (repeat false n)); first done.
+    exfalso.
+    suff: (forallb negb (repeat false n) = true) by congruence.
+    by apply /forallb_forall => a /(@repeat_spec bool) ->.
+  Qed.
+
+
+
+  Lemma almost_eq_truncate_iff l1 l2 : almost_eq l1 l2 <-> truncate l1 = truncate l2.
+  Proof.
+    split.
+    - elim.
+      + move=> a {}l1 {}l2 IH E /=.
+        suff ->: forallb negb l1 = forallb negb l2 by rewrite E.
+        elim: IH {E}.
+        * by move=> > /= _ ->.
+        * by elim; [elim|].
+      + move=> a1 a2. by rewrite !truncate_repeat_false.
+    - move=> E.
+      have := almost_eq_truncate l2.
+      have /almost_eq_sym := almost_eq_truncate l1.
+      rewrite E.
+      by apply: almost_eq_trans.
+  Qed.
+      
+
+  Lemma almost_eq_truncate_tape_iff t1 t2:
+    truncate_tape t1 = truncate_tape t2 <-> almost_eq_tape t1 t2.
+  Proof.
+    split.
+    - move=> E.
+      apply: almost_eq_tape_trans; [|by apply: almost_eq_tape_truncate_tape].
+      apply: almost_eq_tape_sym.
+      apply: almost_eq_tape_trans; [|by apply: almost_eq_tape_truncate_tape].
+      rewrite E.
+      by apply: almost_eq_tape_refl.
+    - move=> E.
+      destruct E. unfold truncate_tape.
+      apply almost_eq_truncate_iff in H, H0.
+      now rewrite H H0.
+  Qed.
+
   #[local] Opaque step.
 
-  Lemma steps_truncate {M k q t} :
+  Lemma steps_truncate_tape_None {M k q t} :
     steps M k (q, truncate_tape t) = None <-> (steps M k (q, t) = None).
   Proof.
     apply: almost_eq_tape_steps_None.
-    apply: almost_eq_tape_truncate_tape.
+    by apply: almost_eq_tape_truncate_tape.
   Qed.
-
-(* TODO MOVE *)
-  Lemma almost_eq_tape_steps_Some M k q q1 q2 t1 t'1 t2 t'2 :
-  almost_eq_tape t1 t2 -> 
-  steps M k (q, t1) = Some (q1, t'1) ->
-  steps M k (q, t2) = Some (q2, t'2) ->
-  q1 = q2 /\ almost_eq_tape t'1 t'2.
-Proof.
-  revert q q1 q2 t1 t'1 t2 t'2.
-  induction k.
-  - intros.
-    split.
-    + injection H0. injection H1. intros. rewrite <- H3. rewrite <- H5. reflexivity.
-    + injection H0. injection H1. intros. rewrite <- H2. rewrite <- H4. apply H.
-  - intros.
-    replace (S k) with (1 + k) in H0 by lia.
-    replace (S k) with (1 + k) in H1 by lia.
-    rewrite steps_plus in H0.
-    rewrite steps_plus in H1.
-    remember (steps M 1 (q, t1)) as s1.
-    remember (steps M 1 (q, t2)) as s2.
-    destruct s1; destruct s2.
-    + simpl in H0. simpl in H1.
-      destruct p as [q''1 t''1]. destruct p0 as [q''2 t''2].
-      specialize (IHk q''1 q1 q2 t''1 t'1 t''2 t'2).
-      assert (E := almost_eq_tape_step_Some).
-      specialize (E M q q''1 q''2 t1 t''1 t2 t''2 H).
-      simpl in Heqs1.
-      simpl in Heqs2.
-      symmetry in Heqs1.
-      symmetry in Heqs2.
-      specialize (E Heqs1).
-      specialize (E Heqs2).
-      destruct E.
-      rewrite <- H2 in H1.
-      specialize (IHk H3 H0 H1).
-      destruct IHk.
-      split.
-      * apply H4.
-      * apply H5.
-    + simpl in H1. inversion H1.
-    + simpl in H0. inversion H0.
-    + simpl in H1. inversion H1.
-Qed.
 
 
 
@@ -294,8 +357,6 @@ Section Construction.
         end).
   Defined.
 
-  Print M'.
-
   #[local] Notation step := (step M').
   #[local] Notation steps := (steps M').
   #[local] Notation state := (state M').
@@ -405,685 +466,80 @@ Section Construction.
     by rewrite /= /step /= construct_trans_spec decode_encode_space ?Hq.
   Qed.
 
+  Lemma almost_eq_tape_step q q' t1 t t' :
+    almost_eq_tape t' t ->
+    step (q, t) = Some (q', t1) ->
+    exists t0, step (q, t') = Some (q', t0) /\ almost_eq_tape t0 t1.
+  Proof.
+    move E: (step (q, t')) => [[q2 t2]|].
+    - move: E => /almost_eq_tape_step_Some /[apply] /[apply].
+      move=> [<-] ?. by eexists.
+    - by move: E => /almost_eq_tape_step_None /[apply] ->.
+  Qed.
+
+  Lemma almost_eq_tape_steps  k q q' t1 t t' :
+    almost_eq_tape t' t ->
+    steps k (q, t) = Some (q', t1) ->
+    exists t0, steps k (q, t') = Some (q', t0) /\ almost_eq_tape t0 t1.
+  Proof.
+    move=> Ht't.
+    elim: k q' t1.
+    - move=> ?? /= [<- <-]. by eexists.
+    - move=> k IH q' t1.
+      have ->: S k = k +1 by lia.
+      rewrite steps_plus /=.
+      move E: (steps k (q, t)) => [[??]|]; last done.
+      move: E => /IH [?] [Hk] /= /almost_eq_tape_step /[apply].
+      move=> [t''] [??].
+      exists t''. split; last done.
+      by rewrite steps_plus Hk.
+  Qed.
+
+  Lemma simulation_output q q' t t' t''':
+    TM.eval M q t q' t' ->
+    almost_eq_tape t''' (encode_tape (Vector.hd t)) ->
+    (exists k l,
+      steps k ((encode_state q), t''') = Some (encode_state q', l) /\
+      steps (S k) ((encode_state q), t''') = None /\
+      almost_eq_tape l ((encode_tape (Vector.hd t')))).
+  Proof.
+    move=> /TM_facts.TM_eval_iff [n].
+    elim: n q t q' t' t'''.
+    { move=> q t q' t' t'''. rewrite /= /TM_facts.haltConf /=.
+      case E: (TM.halt q) => [|]; last done.
+      move: E => /simulation_halt => /(_ t''') H [<- <-] ?.
+      by exists 0, t'''. }
+    move=> n IH q t q' t' t'''. rewrite /= /TM_facts.haltConf /=.
+    case E: (TM.halt q) => [|].
+    { move: E => /simulation_halt => /(_ t''') H [<- <-] ?.
+      by exists 0, t'''. }
+    rewrite (Vector.eta t).
+    move: E => /simulation_step => /(_ (Vector.hd t)) [k1].
+    move: (VectorDef.tl t). apply: Vector.case0.
+    move: (TM_step _) => [q'' ts''].
+    move E: (steps (S k1) _) => [[qk1 tk1]|]; last done.
+    move=> Hk1 /IH /= {}IH.
+    move: E => /almost_eq_tape_steps /[apply] - [t''''].
+    move: Hk1 => /= [->] /almost_eq_truncate_tape_iff /IH [k2] [t'''''].
+    move=> [/[dup] + ->].
+    move=> /almost_eq_tape_steps H'k2 /= [Hk2 ?] [Hk1].
+    move=> /[dup] /H'k2 [t8] [H''k2 ?] ?.
+    exists ((S k1) + k2), t8. rewrite (steps_plus) /= Hk1 /=.
+    split; [done|split].
+    - rewrite H''k2 /=.
+      apply: (almost_eq_tape_step_None M') Hk2.
+      by apply: almost_eq_tape_sym.
+    - apply: almost_eq_tape_trans; eassumption.
+  Qed.
+
   Lemma simulation q t :
     (exists q' t', TM.eval M q t q' t') ->
     exists k, steps k ((encode_state q), (encode_tape (Vector.hd t))) = None.
   Proof.
-    move=> [q'] [t'] /TM_facts.TM_eval_iff [n].
-    elim: n q t.
-    { move=> q t. rewrite /= /TM_facts.haltConf /=.
-      case E: (TM.halt q) => [|]; last done.
-      move: E => /simulation_halt H _.
-      exists 1. by apply: H. }
-    move=> n IH q t. rewrite /= /TM_facts.haltConf /=.
-    case E: (TM.halt q) => [|].
-    { move: E => /simulation_halt H _. exists 1. by apply: H. }
-    rewrite (Vector.eta t).
-    move: E => /simulation_step => /(_ (Vector.hd t)) [k1].
-    move: (VectorDef.tl t). apply: Vector.case0.
-    move: (TM_step _) => [q'' ts''] Hk1 /IH [k2 Hk2] /=.
-    exists ((S k1) + k2). rewrite (steps_plus).
-    move: (encode_state q, _) Hk1 Hk2 => x.
-    move Hk1: (steps (S k1) x) => [[q''' t''']|] /=; last done.
-    move=> [] <- Ht''' /(@steps_truncate M').
-    rewrite -Ht'''. by move=> /steps_truncate.
+    move=> [q'] [t'] /simulation_output => /(_ _ (almost_eq_tape_refl (encode_tape (Vector.hd t)))).
+    move=> [k] [l] [?] [??].
+    by exists (S k).
   Qed.
-
-
-
-Lemma h1 l1 l2 l3 b:
-almost_eq_tape ([], b, l1) (true :: l3, b, l2) -> False.
-Proof.
-  intros.
-  inversion H.
-  inversion H2.
-  induction n2.
-  - inversion H9.
-  - simpl in H9.
-    inversion H9.
-Qed.
-
-
-Lemma h2 l1 l2 l3 b:
-almost_eq_tape (l1, b, []) (l2, b, true :: l3) -> False.
-Proof.
-  intros.
-  inversion H.
-  inversion H6.
-  induction n2.
-  - inversion H9.
-  - simpl in H9.
-    inversion H9.
-Qed.
-
-Lemma h3 l1 l2 l1' l2' b:
-almost_eq_tape (l1, b, l2) (l1', b, l2') -> almost_eq l1 l1' /\ almost_eq l2 l2'.
-Proof.
-  intros.
-  inversion H.
-  auto.
-Qed.
-
-Lemma h4 l:
-almost_eq [] (false :: l) -> exists n, l = repeat false n.
-Proof.
-  intros.
-  inversion H.
-  induction n2.
-  - inversion H2.
-  - simpl in H2.
-    injection H2.
-    intros.
-    rewrite <- H0.
-    exists n2.
-    reflexivity.
-Qed.
-
-Lemma h5 l1 l2:
-almost_eq (true :: l1) (false :: l2) -> False.
-Proof.
-  intros.
-  inversion H.
-  induction n1; inversion H1.
-Qed.
-
-Lemma h6 l1 l2 b:
-almost_eq (b :: l1) (b :: l2) -> almost_eq l1 l2.
-Proof.
-  intros.
-  inversion H.
-  - apply H1.
-  - induction n1, n2.
-    + inversion H1.
-    + inversion H1.
-    + inversion H2.
-    + simpl in H1.
-      simpl in H2.
-      inversion H1.
-      inversion H2.
-      subst.
-      constructor.
-Qed.
-
-Lemma h7 l1 l2 l3 l3' b:
-almost_eq_tape (l1, b, true :: l3) (l2, b, false :: l3') -> False.
-Proof.
-  intros.
-  inversion H.
-  inversion H6.
-  destruct n1; inversion H8.
-Qed.
-
-Lemma hft1 l1 l2 l3 l3' b:
-almost_eq_tape (l1, b, false :: l3) (l2, b, true :: l3') -> False.
-Proof.
-  intros.
-  inversion H.
-  inversion H6.
-  destruct n2; inversion H9.
-Qed.
-
-Lemma htf1 l1 l2 l3 l3' b:
-almost_eq_tape (l1, b, true :: l3) (l2, b, false :: l3') -> False.
-  intros.
-  inversion H.
-  inversion H6.
-  destruct n1; inversion H8.
-Qed.
-
-Lemma htf2 l1 l2 l3 l3' b:
-almost_eq_tape (true :: l1, b, l3) (false :: l2, b, l3') -> False.
-  intros.
-  inversion H.
-  inversion H2.
-  destruct n1; inversion H8.
-Qed.
-
-Lemma hft2 l1 l2 l3 l3' b:
-almost_eq_tape (false :: l1, b, l3) (true :: l2, b, l3') -> False.
-  intros.
-  inversion H.
-  inversion H2.
-  destruct n2; inversion H9.
-Qed.
-
-Lemma htn l1:
-almost_eq (true :: l1) [] -> False.
-  intros.
-  inversion H.
-  destruct n1; inversion H1.
-Qed.
-
-
-
-Lemma almost_eq_step q q' t1 t t' :
-              almost_eq_tape t' t ->
-              step (q, t) = Some (q', t1) ->
-              exists t0, step (q, t') = Some (q', t0) /\ almost_eq_tape t0 t1.
-Proof.
-  intros.
-  destruct (step (q, t')) eqn:H1.
-  - destruct p. 
-    apply almost_eq_tape_sym in H.
-    assert (H2 := almost_eq_tape_step_Some M' _ _ _ _ _ _ _ H H0 H1).
-    destruct H2.
-    rewrite <- H2.
-    exists p.
-    split.
-    + reflexivity.
-    + apply almost_eq_tape_sym in H3. apply H3.
-  - assert (H2 := almost_eq_tape_step_None M' _ _ _ H H1). congruence.
-
-
-  (* intros.
-  unfold step in H0.
-  destruct t.
-  destruct p.
-  destruct (trans' M' (q, b)) eqn:E.
-  - destruct p.
-    destruct p.
-    injection H0.
-    intros.
-    destruct t'.
-    destruct p.
-    destruct b1, b. 2,3: inversion H.
-    + induction l2, l0.
-      * induction l1, l.
-        -- destruct d; simpl in H1; rewrite <- H1; destruct b0; unfold step; rewrite E; rewrite H2; simpl; eexists _; split. 1,3,5,7: now reflexivity. 1,2,3,4: constructor; apply almost_eq_refl.
-        -- destruct b. 1: destruct (h2 [] [] l true H).
-           destruct d; simpl in H1; rewrite <- H1; destruct b0; unfold step; rewrite E; rewrite H2; simpl; eexists _; split. 1,3,5,7: now reflexivity.
-           1,2,3,4: apply h3 in H; destruct H as [H' H'']; constructor. 1,3,5,7: repeat constructor; apply H'. 1,2: constructor; apply H''. 1,2:   apply h4 in H''; destruct H''; rewrite H; replace [] with (repeat false 0) by easy; constructor.
-        -- destruct a. 1: apply almost_eq_tape_sym in H. 1: destruct (h2 [] [] l1 true H).
-           destruct d; simpl in H1; rewrite <- H1; destruct b0; unfold step; rewrite E; rewrite H2; simpl; eexists _; split. 1,3,5,7: now reflexivity.
-           1,2,3,4: apply h3 in H; destruct H as [H' H'']; constructor. 1,3,5,7: repeat constructor; apply H'. 1,2,3,4: repeat constructor. 1,2: apply H''. 1,2: apply almost_eq_sym in H''; apply h4 in H''; destruct H''; rewrite H; replace [] with (repeat false 0) by easy; constructor.
-        -- destruct d; simpl in H1; rewrite <- H1; destruct b0; unfold step; rewrite E; rewrite H2; simpl; eexists _; split. 1,3,5,7: now reflexivity. 
-        1,2,3,4: apply h3 in H; destruct H as [H' H'']; destruct a, b. 2,6,10,14: apply h5 in H''; destruct H''. 2,5,8,11: apply almost_eq_sym in H''; apply h5 in H''; destruct H''. 1,2,3,4,5,6,7,8: constructor. 1,3,5,7,9,11,13, 15: repeat constructor; apply H'. 1,2,3,4: constructor; apply H''. 1,2,3,4: apply h6 in H''; apply H''.
-        
-           
-    * induction l1, l.
-      -- destruct b. 1: destruct (h1 [] [] l0 true H). destruct d; simpl in H1; rewrite <- H1; destruct b0; unfold step; rewrite E; rewrite H2; simpl; eexists _; split. 1,3,5,7: now reflexivity. 1,2,3,4: apply h3 in H; destruct H as [H' H'']; constructor. 2,4,6,8: repeat constructor; apply H''. 1,2: apply h4 in H'; destruct H'; rewrite H; replace [] with (repeat false 0) by easy; constructor. 1,2: constructor; apply H'.
-      -- destruct b, b1. 1,2: apply h1 in H; destruct H. 1: apply h2 in H; destruct H. destruct d; simpl in H1; rewrite <- H1; destruct b0; unfold step; rewrite E; rewrite H2; simpl; eexists _; split. 1,3,5,7: now reflexivity.
-      1,2,3,4: apply h3 in H; destruct H as [H' H'']; constructor. 2,4: repeat constructor; apply H''. 3,5: repeat constructor; apply H'. 1,2: apply h4 in H'; destruct H'; rewrite H; replace [] with (repeat false 0) by easy; constructor. 1,2: apply h4 in H''; destruct H''; rewrite H; replace [] with (repeat false 0) by easy; constructor.
-      -- destruct a, b. 1,3: apply h1 in H; destruct H. 1: apply almost_eq_tape_sym in H; apply h2 in H; destruct H.
-        destruct d; simpl in H1; rewrite <- H1; destruct b0; unfold step; rewrite E; rewrite H2; simpl; eexists _; split. 1,3,5,7: now reflexivity. 1,2,3,4: apply h3 in H; destruct H as [H' H'']; constructor. 2,4: repeat constructor; apply H''. 3,5: repeat constructor; apply H'. 1,2: apply h4 in H'; destruct H'; rewrite H;replace [] with (repeat false 0) by easy; constructor. 1,2: apply almost_eq_sym in H''; apply h4 in H''; destruct H''; rewrite H;replace [] with (repeat false 0) by easy; constructor.
-      -- destruct a,b,b1. 1,2,5,6: apply h1 in H; destruct H. 2: apply h7 in H; destruct H. 2: apply hft1 in H; destruct H.
-        1,2: destruct d; simpl in H1; rewrite <- H1; destruct b0; unfold step; rewrite E; rewrite H2; simpl; eexists _; split. 1,3,5,7,9,11,13,15: now reflexivity.
-        1,2,3,4,5,6,7,8: apply h3 in H; destruct H as [H' H'']; constructor. 2,4,10,12: constructor; apply H''. 3,5,9,11: constructor; apply H'. 1,2,5,6: apply h4 in H'; destruct H'; rewrite H; replace [] with (repeat false 0) by easy; constructor. 1,2,3,4: apply h6 in H''; apply H''.
-  
-    * induction l1, l.
-      --   destruct a. 1: apply almost_eq_tape_sym in H; apply h1 in H; destruct H.
-        1: destruct d; simpl in H1; rewrite <- H1; destruct b0; unfold step; rewrite E; rewrite H2; simpl; eexists _; split. 1,3,5,7: now reflexivity. 
-        1,2,3,4: apply h3 in H; destruct H as [H' H'']; constructor. 2,4,6,8: repeat constructor; apply H''. 1,2: apply almost_eq_sym in H'; apply h4 in H'; destruct H'; rewrite H; replace [] with (repeat false 0) by easy; constructor. 1,2: constructor; apply H'.
-      -- destruct a, b. 1,3: apply h2 in H; destruct H. 1: apply almost_eq_tape_sym in H; apply h1 in H; destruct H.
-        destruct d; simpl in H1; rewrite <- H1; destruct b0; unfold step; rewrite E; rewrite H2; simpl; eexists _; split. 1,3,5,7: now reflexivity.
-         1,2,3,4: apply h3 in H; destruct H as [H' H'']; constructor. 2,4: constructor; apply H''. 3,5: constructor; apply H'. 1,2: apply almost_eq_sym in H'; apply h4 in H'; destruct H'; rewrite H; replace [] with (repeat false 0) by easy; constructor. 1,2: apply h4 in H''; destruct H''; rewrite H; replace [] with (repeat false 0) by easy; constructor.
-      -- destruct a, a0; apply almost_eq_tape_sym in H. 1,2: apply h1 in H; destruct H. 1: apply h2 in H; destruct H.
-        1: destruct d; simpl in H1; rewrite <- H1; destruct b0; unfold step; rewrite E; rewrite H2; simpl; eexists _; split. 1,3,5,7: now reflexivity. 
-        1,2,3,4: apply h3 in H; destruct H as [H' H'']; apply almost_eq_tape_sym; constructor. 2,4: constructor; apply H''. 3,5: constructor; apply H'. 1,2: apply h4 in H'; destruct H'; rewrite H; replace [] with (repeat false 0) by easy; constructor. 1,2: apply h4 in H''; destruct H''; rewrite H; replace [] with (repeat false 0) by easy; constructor.
-      -- destruct a, a0, b. 2,3,4: apply almost_eq_tape_sym in H; apply h1 in H; destruct H. 1: apply almost_eq_tape_sym in H; apply h1 in H; destruct H. 2: apply h3 in H; destruct H as [H' H'']; apply h5 in H''; destruct H''. 2: apply almost_eq_tape_sym in H; apply h3 in H; destruct H as [H' H'']; apply h5 in H''; destruct H''.
-        1,2: destruct d; simpl in H1; rewrite <- H1; destruct b0; unfold step; rewrite E; rewrite H2; simpl; eexists _; split. 1,3,5,7,9,11,13,15: now reflexivity. 
-         1,2,3,4,5,6,7,8: apply h3 in H; destruct H as [H' H'']; constructor. 2,4,10,12: constructor; apply H''. 3,5,9,11: constructor; apply H'. 1,2,5,6: apply almost_eq_sym in H'; apply h4 in H'; destruct H'; rewrite H; replace [] with (repeat false 0) by easy; constructor. 1,2,3,4: apply h6 in H''; apply H''.
-
-    * induction l1, l.
-      -- destruct a, b. 2: apply htf2 in H; destruct H. 2: apply hft2 in H; destruct H.
-         1,2: destruct d; simpl in H1; rewrite <- H1; destruct b0; unfold step; rewrite E; rewrite H2; simpl; eexists _; split. 1,3,5,7,9,11,13,15: now reflexivity. 
-         1,2,3,4,5,6,7,8: apply h3 in H; destruct H as [H' H'']; constructor.
-         2,4,10,12: repeat constructor; apply H''. 3,5,9,11: constructor; apply H'. 3,4,7,8: apply H''. 1,2,3,4: apply h6 in H'; apply H'.
-      -- destruct a,b,b1. 1,3,5,7: apply h2 in H; destruct H. 2: apply htf2 in H; destruct H. 2: apply hft2 in H; destruct H.
-        1,2: destruct d; simpl in H1; rewrite <- H1; destruct b0; unfold step; rewrite E; rewrite H2; simpl; eexists _; split. 1,3,5,7,9,11,13,15: now reflexivity. 
-        1,2,3,4,5,6,7,8: apply h3 in H; destruct H as [H' H'']; constructor.
-        2,4,10,12: constructor; apply H''. 3,5,9,11: constructor; apply H'. 1,2,5,6: apply h6 in H'; apply H'. 1,2,3,4: apply h4 in H''; destruct H''; rewrite H; replace [] with (repeat false 0) by easy; constructor.
-      -- destruct a, a0, b. 2,4: apply htf2 in H; destruct H. 3,5: apply hft2 in H; destruct H. 1,3: apply almost_eq_tape_sym in H; apply h2 in H; destruct H.
-        1,2: destruct d; simpl in H1; rewrite <- H1; destruct b0; unfold step; rewrite E; rewrite H2; simpl; eexists _; split. 1,3,5,7,9,11,13,15: now reflexivity.
-        1,2,3,4,5,6,7,8: apply h3 in H; destruct H as [H' H'']; constructor.
-         2,4,10,12: repeat constructor; apply H''. 3,5,9,11: constructor; apply H'. 3,4,7,8: apply almost_eq_sym in H''; apply h4 in H''; destruct H''; rewrite H; replace [] with (repeat false 0) by easy; constructor.
-         1,2,3,4: apply h6 in H'; apply H'.
-      --  destruct a, a0, b, b1. 2,4,10,12: apply htf1 in H; destruct H. 2,5,6: apply htf2 in H; destruct H. 2: apply hft1 in H; destruct H. 3,5,6: apply hft2 in H; destruct H. 4: apply hft1 in H; destruct H.
-        1,2,3,4: destruct d; simpl in H1; rewrite <- H1; destruct b0; unfold step; rewrite E; rewrite H2; simpl; eexists _; split. 1,3,5,7,9,11,13,15,17,19,21,23,25,27,29,31: now reflexivity.
-        1,2,3,4,5,6,7,8,9,10,11,12,13,14,15,16:
-        apply h3 in H; destruct H as [H' H'']; constructor.
-        2,4,10,12,18,20,26,28: constructor; apply H''.
-        3,5,9,11,15,17,21,23: constructor; apply H'.
-        1,2,5,6,9,10,13,14: apply h6 in H'; apply H'.
-        1,2,3,4,5,6,7,8: apply h6 in H''; apply H''.
-
-
-
-    + induction l2, l0.
-      * induction l1, l.
-        -- destruct d; simpl in H1; rewrite <- H1; destruct b0; unfold step; rewrite E; rewrite H2; simpl; eexists _; split. 1,3,5,7: now reflexivity. 1,2,3,4: constructor; apply almost_eq_refl.
-        -- destruct b. 1: apply h2 in H; destruct H.
-           destruct d; simpl in H1; rewrite <- H1; destruct b0; unfold step; rewrite E; rewrite H2; simpl; eexists _; split. 1,3,5,7: now reflexivity.
-           1,2,3,4: apply h3 in H; destruct H as [H' H'']; constructor. 1,3,5,7: repeat constructor; apply H'. 1,2: constructor; apply H''. 1,2:   apply h4 in H''; destruct H''; rewrite H; replace [] with (repeat false 0) by easy; constructor.
-        -- destruct a. 1: apply almost_eq_tape_sym in H. 1: apply h2 in H; destruct H.
-           destruct d; simpl in H1; rewrite <- H1; destruct b0; unfold step; rewrite E; rewrite H2; simpl; eexists _; split. 1,3,5,7: now reflexivity.
-           1,2,3,4: apply h3 in H; destruct H as [H' H'']; constructor. 1,3,5,7: repeat constructor; apply H'. 1,2,3,4: repeat constructor. 1,2: apply H''. 1,2: apply almost_eq_sym in H''; apply h4 in H''; destruct H''; rewrite H; replace [] with (repeat false 0) by easy; constructor.
-        -- destruct d; simpl in H1; rewrite <- H1; destruct b0; unfold step; rewrite E; rewrite H2; simpl; eexists _; split. 1,3,5,7: now reflexivity. 
-        1,2,3,4: apply h3 in H; destruct H as [H' H'']; destruct a, b. 2,6,10,14: apply h5 in H''; destruct H''. 2,5,8,11: apply almost_eq_sym in H''; apply h5 in H''; destruct H''. 1,2,3,4,5,6,7,8: constructor. 1,3,5,7,9,11,13, 15: repeat constructor; apply H'. 1,2,3,4: constructor; apply H''. 1,2,3,4: apply h6 in H''; apply H''.
-      * induction l1, l.
-        -- destruct b. 1: apply h1 in H; destruct H. destruct d; simpl in H1; rewrite <- H1; destruct b0; unfold step; rewrite E; rewrite H2; simpl; eexists _; split. 1,3,5,7: now reflexivity. 1,2,3,4: apply h3 in H; destruct H as [H' H'']; constructor. 2,4,6,8: repeat constructor; apply H''. 1,2: apply h4 in H'; destruct H'; rewrite H; replace [] with (repeat false 0) by easy; constructor. 1,2: constructor; apply H'.
-        -- destruct b, b1. 1,2: apply h1 in H; destruct H. 1: apply h2 in H; destruct H. destruct d; simpl in H1; rewrite <- H1; destruct b0; unfold step; rewrite E; rewrite H2; simpl; eexists _; split. 1,3,5,7: now reflexivity.
-      1,2,3,4: apply h3 in H; destruct H as [H' H'']; constructor. 2,4: repeat constructor; apply H''. 3,5: repeat constructor; apply H'. 1,2: apply h4 in H'; destruct H'; rewrite H; replace [] with (repeat false 0) by easy; constructor. 1,2: apply h4 in H''; destruct H''; rewrite H; replace [] with (repeat false 0) by easy; constructor.
-        -- destruct a, b. 1,3: apply h1 in H; destruct H. 1: apply almost_eq_tape_sym in H; apply h2 in H; destruct H.
-        destruct d; simpl in H1; rewrite <- H1; destruct b0; unfold step; rewrite E; rewrite H2; simpl; eexists _; split. 1,3,5,7: now reflexivity. 1,2,3,4: apply h3 in H; destruct H as [H' H'']; constructor. 2,4: repeat constructor; apply H''. 3,5: repeat constructor; apply H'. 1,2: apply h4 in H'; destruct H'; rewrite H;replace [] with (repeat false 0) by easy; constructor. 1,2: apply almost_eq_sym in H''; apply h4 in H''; destruct H''; rewrite H;replace [] with (repeat false 0) by easy; constructor.
-        --  destruct a,b,b1. 1,2,5,6: apply h1 in H; destruct H. 2: apply h7 in H; destruct H. 2: apply hft1 in H; destruct H.
-        1,2: destruct d; simpl in H1; rewrite <- H1; destruct b0; unfold step; rewrite E; rewrite H2; simpl; eexists _; split. 1,3,5,7,9,11,13,15: now reflexivity.
-        1,2,3,4,5,6,7,8: apply h3 in H; destruct H as [H' H'']; constructor. 2,4,10,12: constructor; apply H''. 3,5,9,11: constructor; apply H'. 1,2,5,6: apply h4 in H'; destruct H'; rewrite H; replace [] with (repeat false 0) by easy; constructor. 1,2,3,4: apply h6 in H''; apply H''.
-      * induction l1, l.
-        -- destruct a. 1: apply almost_eq_tape_sym in H; apply h1 in H; destruct H.
-        1: destruct d; simpl in H1; rewrite <- H1; destruct b0; unfold step; rewrite E; rewrite H2; simpl; eexists _; split. 1,3,5,7: now reflexivity. 
-        1,2,3,4: apply h3 in H; destruct H as [H' H'']; constructor. 2,4,6,8: repeat constructor; apply H''. 1,2: apply almost_eq_sym in H'; apply h4 in H'; destruct H'; rewrite H; replace [] with (repeat false 0) by easy; constructor. 1,2: constructor; apply H'.
-        -- destruct a, b. 1,3: apply h2 in H; destruct H. 1: apply almost_eq_tape_sym in H; apply h1 in H; destruct H.
-        destruct d; simpl in H1; rewrite <- H1; destruct b0; unfold step; rewrite E; rewrite H2; simpl; eexists _; split. 1,3,5,7: now reflexivity.
-         1,2,3,4: apply h3 in H; destruct H as [H' H'']; constructor. 2,4: constructor; apply H''. 3,5: constructor; apply H'. 1,2: apply almost_eq_sym in H'; apply h4 in H'; destruct H'; rewrite H; replace [] with (repeat false 0) by easy; constructor. 1,2: apply h4 in H''; destruct H''; rewrite H; replace [] with (repeat false 0) by easy; constructor.
-        -- destruct a, a0; apply almost_eq_tape_sym in H. 1,2: apply h1 in H; destruct H. 1: apply h2 in H; destruct H.
-        1: destruct d; simpl in H1; rewrite <- H1; destruct b0; unfold step; rewrite E; rewrite H2; simpl; eexists _; split. 1,3,5,7: now reflexivity. 
-        1,2,3,4: apply h3 in H; destruct H as [H' H'']; apply almost_eq_tape_sym; constructor. 2,4: constructor; apply H''. 3,5: constructor; apply H'. 1,2: apply h4 in H'; destruct H'; rewrite H; replace [] with (repeat false 0) by easy; constructor. 1,2: apply h4 in H''; destruct H''; rewrite H; replace [] with (repeat false 0) by easy; constructor.
-        -- destruct a, a0, b. 2,3,4: apply almost_eq_tape_sym in H; apply h1 in H; destruct H. 1: apply almost_eq_tape_sym in H; apply h1 in H; destruct H. 2: apply h3 in H; destruct H as [H' H'']; apply h5 in H''; destruct H''. 2: apply almost_eq_tape_sym in H; apply h3 in H; destruct H as [H' H'']; apply h5 in H''; destruct H''.
-        1,2: destruct d; simpl in H1; rewrite <- H1; destruct b0; unfold step; rewrite E; rewrite H2; simpl; eexists _; split. 1,3,5,7,9,11,13,15: now reflexivity. 
-         1,2,3,4,5,6,7,8: apply h3 in H; destruct H as [H' H'']; constructor. 2,4,10,12: constructor; apply H''. 3,5,9,11: constructor; apply H'. 1,2,5,6: apply almost_eq_sym in H'; apply h4 in H'; destruct H'; rewrite H; replace [] with (repeat false 0) by easy; constructor. 1,2,3,4: apply h6 in H''; apply H''.
-      * induction l1, l.
-        -- destruct a, b. 2: apply htf2 in H; destruct H. 2: apply hft2 in H; destruct H.
-         1,2: destruct d; simpl in H1; rewrite <- H1; destruct b0; unfold step; rewrite E; rewrite H2; simpl; eexists _; split. 1,3,5,7,9,11,13,15: now reflexivity. 
-         1,2,3,4,5,6,7,8: apply h3 in H; destruct H as [H' H'']; constructor.
-         2,4,10,12: repeat constructor; apply H''. 3,5,9,11: constructor; apply H'. 3,4,7,8: apply H''. 1,2,3,4: apply h6 in H'; apply H'.
-        -- destruct a,b,b1. 1,3,5,7: apply h2 in H; destruct H. 2: apply htf2 in H; destruct H. 2: apply hft2 in H; destruct H.
-        1,2: destruct d; simpl in H1; rewrite <- H1; destruct b0; unfold step; rewrite E; rewrite H2; simpl; eexists _; split. 1,3,5,7,9,11,13,15: now reflexivity. 
-        1,2,3,4,5,6,7,8: apply h3 in H; destruct H as [H' H'']; constructor.
-        2,4,10,12: constructor; apply H''. 3,5,9,11: constructor; apply H'. 1,2,5,6: apply h6 in H'; apply H'. 1,2,3,4: apply h4 in H''; destruct H''; rewrite H; replace [] with (repeat false 0) by easy; constructor.
-        -- destruct a, a0, b. 2,4: apply htf2 in H; destruct H. 3,5: apply hft2 in H; destruct H. 1,3: apply almost_eq_tape_sym in H; apply h2 in H; destruct H.
-        1,2: destruct d; simpl in H1; rewrite <- H1; destruct b0; unfold step; rewrite E; rewrite H2; simpl; eexists _; split. 1,3,5,7,9,11,13,15: now reflexivity.
-        1,2,3,4,5,6,7,8: apply h3 in H; destruct H as [H' H'']; constructor.
-         2,4,10,12: repeat constructor; apply H''. 3,5,9,11: constructor; apply H'. 3,4,7,8: apply almost_eq_sym in H''; apply h4 in H''; destruct H''; rewrite H; replace [] with (repeat false 0) by easy; constructor.
-         1,2,3,4: apply h6 in H'; apply H'.
-        -- destruct a, a0, b, b1. 2,4,10,12: apply htf1 in H; destruct H. 2,5,6: apply htf2 in H; destruct H. 2: apply hft1 in H; destruct H. 3,5,6: apply hft2 in H; destruct H. 4: apply hft1 in H; destruct H.
-        1,2,3,4: destruct d; simpl in H1; rewrite <- H1; destruct b0; unfold step; rewrite E; rewrite H2; simpl; eexists _; split. 1,3,5,7,9,11,13,15,17,19,21,23,25,27,29,31: now reflexivity.
-
-        1,2,3,4,5,6,7,8,9,10,11,12,13,14,15,16:
-        apply h3 in H; destruct H as [H' H'']; constructor.
-        2,4,10,12,18,20,26,28: constructor; apply H''.
-        3,5,9,11,15,17,21,23: constructor; apply H'.
-        1,2,5,6,9,10,13,14: apply h6 in H'; apply H'.
-        1,2,3,4,5,6,7,8: apply h6 in H''; apply H''.
-
-    
-
-    - inversion H0. *)
-
-Qed.
-
-
-
-
-
-      
-    
-
-
-
-Lemma almost_eq_steps  k q q' t1 t t' :
-              almost_eq_tape t' t ->
-              steps k (q, t) = Some (q', t1) ->
-              exists t0, steps k (q, t') = Some (q', t0) /\ almost_eq_tape t0 t1.
-Proof.
-  revert q q' t1 t t'.
-  induction k.
-  - intros.
-    simpl.
-    simpl in H0.
-    injection H0.
-    intros.
-    exists t'.
-    rewrite <- H1.
-    rewrite H2.
-    split.
-    + reflexivity. 
-    + apply H.
-  - intros.
-    replace (S k) with (1 + k) in H0 by lia.
-    rewrite steps_plus in H0.
-    destruct (steps 1 (q,t)) eqn:E.
-    2: inversion H0.
-
-    destruct p.
-
-    assert (E2 := almost_eq_step).
-
-  
-    unfold obind in H0.
-    unfold oapp in H0.
-
-
-
-    specialize (E2 q t0 p t t' H E).
-
-    destruct E2. destruct H1.
-
-    specialize (IHk t0 q' t1 p x H2 H0).
-    destruct IHk.
-
-    eexists _.
-    replace (S k) with (1 + k) by lia.
-    rewrite steps_plus.
-    simpl ((steps 1 (q, t'))).
-    rewrite H1.
-
-    unfold obind.
-    unfold oapp.
-
-    apply H3.
-Qed.
-
-
-
-Lemma almost_eq_spec x l:
-almost_eq (repeat false x) l -> exists n, l = repeat false n.
-Proof.
-  intros.
-  revert H.
-  revert x.
-  induction l.
-  - exists 0. reflexivity.
-  - induction x.
-    + destruct a; intros.
-      * inversion H. destruct n2; inversion H2.
-      * simpl in H. apply h4 in H. destruct H. rewrite H. exists (S x). easy.
-    + destruct a; intros.
-      * inversion H. destruct n2; inversion H2.
-      * simpl in H. apply h6 in H. specialize (IHl _ H). destruct IHl. rewrite H0. exists (S x0). easy.
-Qed.
-
-Lemma almost_eq_elim l1 l2 :
-  almost_eq l1 l2 -> 
-  match l1 with
-  | [] => l2 = repeat false (length l2)
-  | a :: l1' =>
-      match l2 with
-      | [] => l1 = repeat false (length l1)
-      | b :: l2' => a = b /\ almost_eq l1' l2'
-      end
-  end.
-Proof.
-  intros H.
-  induction H. 1: done.
-  destruct n1,n2; cbn.
-  - reflexivity.
-  - rewrite repeat_length. reflexivity.
-  - rewrite repeat_length. reflexivity.
-  - repeat constructor.
-Qed.
-
-
-Lemma almost_eq_trans l1 l2 l3 :
-  almost_eq l1 l2 -> almost_eq l2 l3 -> almost_eq l1 l3.
-Proof.
-  intros H.
-  revert l3.
-  induction H.
-  - induction l3.
-    + intros. apply almost_eq_elim in H0. simpl in H0. injection H0. intros. subst. rewrite H1 in H. apply almost_eq_sym in H. apply almost_eq_spec in H. destruct H. rewrite H. replace (false :: repeat false x) with (repeat false (S x)) by easy. replace [] with (repeat false 0) by easy. constructor.
-    + intros. apply almost_eq_elim in H0. destruct H0. subst. constructor. apply IHalmost_eq. apply H1.
-  - intros. apply almost_eq_spec in H. destruct H. rewrite H. constructor.
-
-  (* revert l1 l2 l3.
-  induction l1, l2, l3; intros.
-  - apply H.
-  - apply H0.
-  - replace ([]) with (repeat false 0) by easy.
-    constructor.
-  - destruct b. 1: inversion H; destruct n2; inversion H3.
-    destruct b0. 1: inversion H0; destruct n2; inversion H3.
-    apply h4 in H. destruct H. rewrite H in H0. inversion H0. 2: replace ([]) with (repeat false 0) by easy; constructor.
-
-    apply almost_eq_spec in H2. destruct H2. rewrite H2. replace (false :: repeat false x0) with (repeat false (S x0)) by easy. replace ([]) with (repeat false 0) by easy. constructor.
-  
-  - apply H.
-  - destruct a. 1: inversion H; destruct n1; inversion H2.
-    destruct b. 1: inversion H0; destruct n2; inversion H3.
-    apply almost_eq_cons.
-    apply h4 in H0. destruct H0. apply almost_eq_sym in H. apply h4 in H. destruct H. rewrite H H0. constructor.
-  - destruct a, b. 1,3: inversion H0; destruct n1; inversion H2.
-    1: inversion H; destruct n1; inversion H2.
-    apply almost_eq_sym in H0. apply h4 in H0. destruct H0. rewrite H0 in H. apply h6 in H. apply almost_eq_sym in H. apply almost_eq_spec in H. destruct H. rewrite H. replace (false :: repeat false x0) with (repeat false (S x0)) by easy. replace ([]) with (repeat false 0) by easy. constructor.
-  - destruct a, b, b0. 2,6: inversion H0; destruct n1; inversion H2. 2,5: inversion H0; destruct n2; inversion H3. 2: inversion H; destruct n1; inversion H2. 2: inversion H; destruct n2; inversion H3.
-    1,2: apply h6 in H; apply h6 in H0; constructor; specialize (IHl1 _ _ H H0); apply IHl1. *)
-Qed.
-    
-    
-Lemma almost_eq_tape_trans t1 t2 t3 :
-  almost_eq_tape t1 t2 -> almost_eq_tape t2 t3 -> almost_eq_tape t1 t3.
-Proof.
-  intros.
-  destruct t1, t2, t3; destruct p, p0, p1.
-  destruct b, b0, b1.
-  2,3,6,7: inversion H0. 2,3: inversion H. 1,2: apply h3 in H; destruct H; apply h3 in H0; destruct H0; assert (T1 := almost_eq_trans _ _ _ H H0); assert (T2 := almost_eq_trans _ _ _ H1 H2); constructor. 1,3: apply T1. 1,2: apply T2.
-Qed.
-
-
-
-(* TODO used dependent destruction here*)
-Require Import Coq.Program.Equality.
-
-Lemma vector_rewrite (t : Vector.t (TM.tape (finType_CS bool)) 1) : | Vector.hd t | = t.
-Proof.
-  dependent destruction t.
-  cbn.
-  dependent destruction t.
-  reflexivity.
-Qed.
-
-  
-
-
-Lemma truncate_almost_eq t1 t2:
-truncate_tape t1 = truncate_tape t2 -> almost_eq_tape t1 t2.
-Proof.
-  intros.
-  assert (H1 := almost_eq_tape_truncate_tape t1).
-  assert (H2 := almost_eq_tape_truncate_tape t2).
-  rewrite H in H1.
-  apply almost_eq_tape_sym in H1.
-  assert (T := almost_eq_tape_trans).
-  specialize (T _ _ _ H1 H2).
-  apply T.
-Qed.
-
-
-Lemma simulation_output q q' t t' t''':
-  TM.eval M q t q' t' ->
-  almost_eq_tape t''' (encode_tape (Vector.hd t)) ->
-  (exists k l, steps k ((encode_state q), t''') = Some (encode_state q', l)
-  /\
-  steps (S k) ((encode_state q), t''') = None /\
-  almost_eq_tape l ((encode_tape (Vector.hd t')))
-  ).
-Proof.
-  intros H.
-
-  (* destruct H as [q' H]. *)
-  rewrite TM_facts.TM_eval_iff in H.
-  destruct H as [n H].
-
-  revert q q' t t' t''' H.
-
-  induction n.
-  - intros.
-    simpl in H.
-    destruct (TM_facts.haltConf (TM_facts.mk_mconfig q t)) eqn:H1.
-    + inversion H.
-      exists 0.
-      (* exists (encode_state q'). *)
-      exists (t''').
-      simpl.
-      split.
-      * reflexivity.
-      * split.
-        -- assert (X := simulation_halt).
-           unfold TM_facts.haltConf in H1.
-           unfold TM_facts.cstate in H1.
-           specialize (X _ t''' H1).
-           rewrite <- H3.
-           apply X.
-        -- rewrite <- H4. apply H0. 
-    + inversion H.
-  - intros.
-
-      destruct (TM.halt q) eqn:H1.
-      
-      + simpl in H.
-        unfold TM_facts.haltConf in H.
-        unfold TM_facts.cstate in H.
-        rewrite H1 in H.
-        injection H.
-        intros.
-        
-        exists 0.
-        (* exists (encode_state q). *)
-        exists (t''').
-        simpl.
-        split.
-        * rewrite H3. reflexivity.
-        * split.
-          -- assert (X := simulation_halt).
-            specialize (X _ t''' H1).
-            apply X.
-
-          -- rewrite <- H2. apply H0.
-      
-      +
-
-        assert (U4 : TM_facts.loopM (TM_facts.mk_mconfig q t) (S n) =
-        TM_facts.loopM (TM_step (TM_facts.mk_mconfig q t)) n).
-        
-        * unfold TM_facts.loopM.
-          unfold Prelim.loop.
-          unfold TM_facts.haltConf.
-          unfold TM_facts.cstate.
-          rewrite H1.
-          reflexivity.
-
-        *
-          rewrite U4 in H.
-    
-          assert (H2 := simulation_step).
-          specialize (H2 q (Vector.hd t) H1).
-          destruct H2 as [k H2].
-
-          rewrite (vector_rewrite t) in H2.
-
-    
-          destruct (TM_step (TM_facts.mk_mconfig q t)) as [q'' t''].
-
-          unfold omap in H2.
-          unfold obind in H2.
-          unfold oapp in H2.
-          unfold encode_config in H2.
-
-
-          destruct (steps (S k) (encode_state q, encode_tape (Vector.hd t))) eqn:Heq in H.
-            -- 
-
-            rewrite Heq in H2.
-            
-            destruct p.
-            inversion H2.
-            subst.
-            (* injection H4. *)
-            intros.
-            (* rewrite H5 in Heq. *)
-            
-            simpl.
-
-            (* assert (Y :
-              almost_eq_tape t''' (encode_tape (Vector.hd t)) ->
-              almost_eq_tape p (encode_tape (Vector.hd t'')) ->
-              steps (S k) (encode_state q, encode_tape (Vector.hd t)) =
-Some (encode_state q'', p) ->
-
-
-              exists t0, steps (S k) (encode_state q, t''') = Some (encode_state q'', t0) /\ almost_eq_tape t0 p
-              
-            
-            
-            ). *)
-
-            assert (Y := almost_eq_steps).
-            specialize (Y _ _ _ _ _ _ H0 Heq).
-            destruct Y.
-            destruct H3.
-
-            assert (T1 := truncate_almost_eq _ _ H5).
-            assert (Z := almost_eq_tape_trans _ _ _ H4 T1).
-
-            specialize (IHn q'' q' t'' t' x H Z).
-
-            destruct IHn as [k0 IHn].
-            (* destruct IHn as [q'0 IHn]. *)
-            destruct IHn as [l IHn].
-            destruct IHn as [IHn1 IHn2].
-            destruct IHn2 as [IHn2 IHn3].
-
-            exists ((S k) + k0).
-            (* exists q'0. *)
-            exists l.
-
-            split.
-            ++ assert (U := @SBTM_facts.steps_plus).
-            specialize (U M' (S k) k0 ((encode_state q, t'''))).
-
-            rewrite U.
-
-            (* rewrite Heq. But these are almost_eq by H0 *)
-
-
-
-            rewrite H3.
-            simpl.
-
-            apply IHn1.
-            ++ split.
-              ** unfold steps.
-                rewrite <- Nat.iter_succ.
-                replace (S (S k + k0)) with (S k + S k0) by lia.
-
-               
-               assert (U := @SBTM_facts.steps_plus).
-            specialize (U M' (S k) (S k0) ((encode_state q, t'''))).
-              
-
-              replace (steps (S k + S k0) (encode_state q, t''')) with (Nat.iter (S k + S k0) (SBTM.obind step) (Some (encode_state q, t'''))) in U by easy.
-              rewrite U.
-              rewrite H3.
-              unfold obind.
-              unfold oapp.
-              apply IHn2.
-
-
-
-
-
-
-
-
-              ** apply IHn3.
-
-
-            
-
-            -- 
-            
-            
-               rewrite Heq in H2.
-               inversion H2.
-
-
-Qed.
-
-  
-
-
-
-
 
   Lemma inverse_simulation q t k :
     steps k ((encode_state q), (encode_tape (Vector.hd t))) = None ->
@@ -1097,549 +553,20 @@ Qed.
     move=> [k1].
     move Hk1: (steps (S k1) _) => [[q' t']|]; last done.
     move=> [] Hq't'.
-    move: Hk1 => /steps_sync H /H{H} /steps_truncate.
+    move: Hk1 => /steps_sync H /H{H} /steps_truncate_tape_None.
     move E: (TM_step _) Hq't' => [q'' t''].
-    move=> [] -> -> /steps_truncate /IH.
+    move=> [] -> -> /steps_truncate_tape_None /IH.
     move=> [q'''] [t'''] /TM_facts.TM_eval_iff [n Hn].
     exists q''', t'''. apply /TM_facts.TM_eval_iff. exists (S n).
     rewrite /= /TM_facts.haltConf Hq -Hn -E (Vector.eta t) /=.
     move: (Vector.tl t). by apply: Vector.case0.
   Qed.
 
-
-
-
-
-
-
-(* Lemma test q q' (t : Vector.t (TM.tape (finType_CS bool)) 1) t'' t''' k :
-  let (q'', t_step) := (TM_step (TM_facts.mk_mconfig q t)) in
-  steps k ((encode_state q), t'') = Some (encode_state q', t''') ->
-  steps (S k) ((encode_state q), t'') = None -> 
-  almost_eq_tape t'' (encode_tape (Vector.hd t)) ->
-  exists t2' k1 k2,
-  steps k1 ((encode_state q), t'') = Some ((encode_state q''), t2') /\ 
-  almost_eq_tape t2' (encode_tape (Vector.hd t_step)) /\
-  steps k2 ((encode_state q''), t2') = Some (encode_state q', t''') /\
-  steps (S k2) ((encode_state q''), t2') = None /\
-  k1 + k2 = k.
-Proof.
-  revert q q' t t'' t'''.
-  assert (I := ax_nat_lt_ind).
-  specialize ( I (fun k => 
-    forall (q q' : TM.state M)
-  (t : Vector.t (TM.tape (finType_CS bool)) 1)
-  (t'' t''' : tape),
-let (q'', t_step) :=
-  TM_step (TM_facts.mk_mconfig q t) in
-steps k (encode_state q, t'') =
-Some (encode_state q', t''') ->
-steps (S k) (encode_state q, t'') = None ->
-almost_eq_tape t'' (encode_tape (Vector.hd t)) ->
-exists (t2' : tape) (k1 k2 : nat),
-  steps k1 (encode_state q, t'') =
-Some (encode_state q'', t2') /\
-almost_eq_tape t2' (encode_tape (Vector.hd t_step)) /\
-steps k2 (encode_state q'', t2') =
-Some (encode_state q', t''') /\
-steps (S k2) (encode_state q'', t2') = None /\
-k1 + k2 = k
-  )).
-
-  apply I.
-  clear I.
-  intros.
-  destruct n.
-  - admit.
-  - destruct (TM_step (TM_facts.mk_mconfig q t)) as [q'' t_step] eqn:Y.
-    intros.
-
-    assert (X := simulation_step).
-    specialize (X q (Vector.hd t)).
-    assert (TM.halt q = false) by admit.
-    specialize (X H3).
-    rewrite vector_rewrite in X.
-    rewrite Y in X.
-    unfold encode_config in X.
-    destruct X as [k0 X].
-
-    eexists _.
-    eexists (S k0).
-    eexists _.
-
-    destruct (steps (S k0)
-  (encode_state q, encode_tape (Vector.hd t))) eqn:N.
-    2: admit.
-
-
-
-
-
-Admitted. *)
-
-Print TM_config.
-
-(* Lemma t n k0 q q' t t':
-  steps n (encode_state q, encode_tape t) = Some (q', t') ->
-  steps (S n) (encode_state q, encode_tape t) = None ->
-  steps (S k0) (encode_state q, encode_tape t) = Some (encode_config (TM_step (TM_facts.mk_mconfig q (| t |)))) -> S k0 <= n.
-Proof.
-  revert q q' t t' k0.
-
-  assert (I := ax_nat_lt_ind).
-  specialize ( I (fun n => 
-
-  forall (q : TM.state M) (q' : state)
-  (t : TM.tape (finType_CS bool)) (t' : tape) (k0 : nat),
-steps n (encode_state q, encode_tape t) = Some (q', t') ->
-steps (S n) (encode_state q, encode_tape t) = None ->
-steps (S k0) (encode_state q, encode_tape t) =
-Some
-  (encode_config
-  (TM_step (TM_facts.mk_mconfig q (| t |)))) ->
-S k0 <= n
-
-  )).
-
-  apply I.
-  clear I.
-  intros.
-  destruct n0.
-  + admit.
-Admitted. *)
-
-  
-  
-
-  
-(* Axiom (ax_nat_lt_ind : forall (P : nat -> Prop),
-       (forall (n : nat), (forall m, m < n -> P m) -> P n) ->
-       forall (n : nat), P n).
-
-
-Lemma inverse_simulation_output q q' t t'' t''' k :
-
-  steps k (encode_state q, t'') = Some (encode_state q', t''') ->
-  steps (S k) (encode_state q, t'') = None ->
-  almost_eq_tape t'' (encode_tape (Vector.hd t)) ->
-  exists t', (TM.eval M q t q' t' /\ almost_eq_tape t''' (encode_tape (Vector.hd t'))).
-Proof.
-
-  revert q q' t t'' t'''.
-
-
-  induction k1 using (Nat.measure_induction _ (fun x => x)).
-  induction k1 using lt_wf_ind. (* Arith importieren *)
-
-  assert (I := ax_nat_lt_ind).
-  specialize ( I (fun k => 
-  
-    forall (q q' : TM.state M)
-  (t : Vector.t (TM.tape (finType_CS bool)) 1)
-  (t'' t''' : tape),
-steps k (encode_state q, t'') =
-Some (encode_state q', t''') ->
-steps (S k) (encode_state q, t'') = None ->
-almost_eq_tape t'' (encode_tape (Vector.hd t)) ->
-exists t' : Vector.t (TM.tape (finType_CS bool)) 1,
-  TM.eval M q t q' t' /\
-almost_eq_tape t''' (encode_tape (Vector.hd t'))
-  
-  )).
-
-  apply I.
-  clear I.
-  intros.
-  destruct n.
-  - clear H.
-
-    destruct (TM.halt q) eqn:H3.
-    + simpl in H0.
-      injection H0.
-      intros.
-      exists t.
-      assert (q = q') by admit.
-      rewrite <- H5.
-      split.
-      * constructor. apply H3.
-      * rewrite <- H. apply H2.
-
-
-
-
-
-
-
-
-
-    + 
-      assert (Y := @almost_eq_tape_steps_None).
-      specialize (Y M' 1 (encode_state q) _ _ H2).
-      rewrite Y in H1.
-    
-      assert (X := simulation_step).
-      specialize (X q (Vector.hd t) H3).
-      destruct X.
-      rewrite vector_rewrite in H.
-
-      assert (Z := @steps_None_mono).
-      specialize (Z M' (encode_state q, encode_tape (Vector.hd t)) (S x) 1 H1).
-      assert (1 <= S x) by lia.
-      specialize (Z H4).
-      rewrite Z in H.
-      cbn in H.
-      inversion H.
-
-
-
-
-
-
-
-
-
-
-  -
-    assert (X := simulation_step).
-    specialize (X q (Vector.hd t)).
-    destruct (TM.halt q) eqn:H3.
-    + 
-    assert (J := simulation_halt).
-    specialize (J q t'' H3).
-    assert (P := @steps_None_mono).
-    specialize (P M' (encode_state q, t'') (S n) 1 J).
-    assert (U : 1 <= S n) by lia.
-    specialize (P U).
-    rewrite P in H0.
-    inversion H0.
-
-    +
-    specialize (X eq_refl).
-    destruct X as [k0 X].
-    rewrite vector_rewrite in X.
-
-
-
-
-
-    destruct (TM_step (TM_facts.mk_mconfig q t)) as [q_step t_step] eqn:V.
-    unfold encode_config in X.
-
-    destruct ((steps (S k0)
-  (encode_state q, encode_tape (Vector.hd t)))) eqn:B. 
-  
-    2: cbn in X; inversion X.
-
-
-    destruct p as [q_des t_des].
-    simpl in X.
-    inversion X.
-
-
-
-
-    rewrite H5 in B.
-
-
-
-
-
-
-
-
-
-  assert (Y := almost_eq_steps).
-
-  specialize (Y (S k0) (encode_state q) (encode_state q_step) t_des (encode_tape (Vector.hd t)) t'' H2 B).
-
-  destruct Y as [t_step' Y].
-  destruct Y as [Y1 Y2].
-
-
-        remember (S n - S k0) as k1 eqn:Ek1.
-    
-    assert (k1 < S n) by lia.
-    assert (S k0 <= S n) by admit.
-    assert (S k0 + k1 = S n) by lia.
-    specialize (H k1).
-    specialize (H H4).
-
-        rewrite <- H8 in H0.
-    rewrite steps_plus in H0.
-
-  rewrite Y1 in H0.
-  simpl in H0.
-
-  specialize (H q_step q' t_step t_step' t''' H0).
-
-
-  rewrite <- H8 in H1.
-  replace (S (S k0 + k1)) with (S k0 + S k1) in H1 by lia.
-  rewrite steps_plus in H1.
-  rewrite Y1 in H1.
-  unfold obind in H1.
-  unfold oapp in H1.
-
-  assert (C := truncate_almost_eq _ _ H6).
-  assert (D := almost_eq_tape_trans _ _ _ Y2 C).
-
-
-
-
-  specialize (H H1 D).
-
-  destruct H as [t_end H].
-  destruct H as [IH1 IH2].
-
-  exists t_end.
-
-  split.
-  2: apply IH2.
-
-  rewrite TM_facts.TM_eval_iff.
-  rewrite TM_facts.TM_eval_iff in IH1.
-
-  destruct IH1 as [n0 IH1].
-
-  exists (S n0).
-
-  simpl.
-  unfold TM_facts.haltConf.
-  cbn.
-  rewrite H3.
-  rewrite V.
-  apply IH1. *)
-
-
-
-
-
-(* 
-
-  assert (T := test).
-  specialize (T q q' t t'' t''' (S n)).
-  destruct (TM_step (TM_facts.mk_mconfig q t)) as [q'' t_step] eqn:E.
-  specialize (T H0 H1 H2).
-  destruct T as [t2' T].
-  destruct T as [k1 T].
-  destruct T as [k2 T].
-  destruct T as [T1 T2].
-  destruct T2 as [T2 T3].
-  destruct T3 as [T3 T4]. 
-  destruct T4 as [T4 T5]. 
-
-  specialize (H k2).
-  assert (k2 < S n) by admit.
-  specialize (H H3).
-
-  specialize (H _ _ _ _ _ T3 T4 T2).
-
-  destruct H as [t' H].
-  destruct H as [HA HB].
-
-  eexists t'.
-
-  split.
-  + 
-  rewrite TM_facts.TM_eval_iff.
-  rewrite TM_facts.TM_eval_iff in HA.
-
-  destruct HA as [n0 HA].
-
-  exists (S n0).
-
-  simpl.
-
-  destruct (TM_facts.haltConf (TM_facts.mk_mconfig q t)).
-  * admit.
-  * rewrite E.
-    apply HA.
-
-  + apply HB.
-
-
-
-
-
-    
-
-
-
-
-  
-
-
-
-
-
-
-
-
-
-
-
-
-
-
-
-
-  revert q q' t t'' t'''.
-  induction k.
-  - intros.
-    simpl in H0.
-    simpl in H.
-    injection H. intros.
-    assert (q = q') by admit.
-    exists t.
-    subst.
-    destruct (TM.halt q') eqn:H5.
-    + split. 2: apply H1. constructor. apply H5.
-    + assert (H6 := simulation_step).
-      specialize (H6 _ (Vector.hd t) H5).
-      destruct H6.
-      assert (H7 := @almost_eq_tape_steps_None).
-      rewrite (H7 M' 1 (encode_state q') _ _ H1) in H0.
-      assert (H8 := @steps_None_mono).
-      assert (1 <= S x) by lia.
-      specialize (H8 M' _ (S x) _ H0 H4).
-      rewrite H8 in H2.
-      simpl in H2.
-      inversion H2.
-  - intros.
-    destruct (TM.halt q) eqn:H2.
-    + eexists _.
-      assert (H4 := simulation_halt q t'' H2).
-      replace (S k) with (1 + k) in H by lia.
-      rewrite steps_plus in H.
-      simpl in H.
-      rewrite H4 in H.
-      cbn in H.
-      inversion H.
-    + assert (H4 := simulation_step).
-      specialize (H4 q (Vector.hd t) H2).
-      destruct H4.
-      rewrite vector_rewrite in H3.
-
-      destruct (TM_step (TM_facts.mk_mconfig q t)) as [q'' tx] eqn:E.
-
-      unfold omap in H3.
-      unfold obind in H3.
-      unfold oapp in H3.
-      unfold encode_config in H3.
-
-
-
-      destruct (steps (S x) (encode_state q, encode_tape (Vector.hd t))) eqn:Heq in H.
-      -- rewrite Heq in H3.
-         destruct p.
-         inversion H3.
-         clear H3.
-         clear E.
-
-
-
-
-
-
-
-      -- rewrite Heq in H3. inversion H3.
-    
-      
-
-
-
-
-
-
-
-
-
-
-
-
-
-
-
-
-
-  - intros.
-    simpl in H.
-    injection H.
-    intros.
-    eexists t.
-    assert (q = q') by admit.
-    subst.
-    split. 2: apply H0.
-    destruct (TM.halt q') eqn:H3.
-    + constructor. apply H3.
-    + assert (H4 := simulation_step _ (Vector.hd t) H3).
-      destruct H4 as [k H4].
-
-      rewrite (vector_rewrite t) in H4.
-
-      destruct (TM_step (TM_facts.mk_mconfig q' t)) as [q'' t''] eqn:E.
-
-      unfold omap in H4.
-      unfold obind in H4.
-      unfold oapp in H4.
-      unfold encode_config in H4.
-      admit.
-
-
-
-
-
-  - intros.
-    destruct (TM.halt q) eqn:H1.
-    + eexists _.
-      assert (H4 := simulation_halt q t'' H1).
-      replace (S k) with (1 + k) in H by lia.
-      rewrite steps_plus in H.
-      simpl in H.
-      rewrite H4 in H.
-      cbn in H.
-      inversion H.
-    + assert (H4 := simulation_step q (Vector.hd t) H1).
-      destruct H4 as [x H4].
-
-      rewrite (vector_rewrite t) in H4.
-
-      destruct (TM_step (TM_facts.mk_mconfig q t)) as [q'' tx] eqn:E.
-
-      unfold omap in H4.
-      unfold obind in H4.
-      unfold oapp in H4.
-      unfold encode_config in H4.
-
-
-
-      destruct (steps (S x) (encode_state q, encode_tape (Vector.hd t))) eqn:Heq in H.
-      -- rewrite Heq in H4.
-         destruct p.
-         inversion H4.
-
-
-
-
-
-      -- rewrite Heq in H4. inversion H4. *)
-
-
-
-  (* Admitted. *)
-    
-    
-
-
-    
-
-
 End Construction.
 
 Require Import Undecidability.Synthetic.Definitions.
 Require Import Undecidability.Synthetic.ReducibilityFacts.
 Require Undecidability.TM.Reductions.Arbitrary_to_Binary.
-
 
 (* TODO existentially quantified q' *)
 Lemma SBTM_simulation (M : TM.TM (finType_CS bool) 1) :
@@ -1649,31 +576,20 @@ Lemma SBTM_simulation (M : TM.TM (finType_CS bool) 1) :
          SBTM_facts.almost_eq_tape t'' (encode_tape (Vector.hd t)) ->
          exists k q' t''', (SBTM.steps M' k (q_start, t'') = Some (q', t''') /\
          SBTM.steps M' (S k) (q_start, t'') = None /\
-         almost_eq_tape t'''  (encode_tape (Vector.hd t')))))
-        
-        /\
+         almost_eq_tape t'''  (encode_tape (Vector.hd t'))))) /\
         (forall t, (exists k, SBTM.steps M' k (q_start, (encode_tape (Vector.hd t))) = None) -> (exists q' t', TM.eval M (TM.start M) t q' t'))}}.
 Proof.
   exists (M' M).
   exists ((encode_space M (space_base M (TM.start M)))).
   split.
-  - intros.
-    assert (U := simulation_output).
-    specialize (U M (TM.start M) q t t' t'' H H0).
-    destruct U.
-    destruct H1.
-    eexists _.
-    eexists _.
-    eexists _.
+  - intros q t t' t'' H H0.
+    destruct (simulation_output M (TM.start M) q t t' t'' H H0) as [k [l H1]].
+    eexists _, _ , _.
     apply H1.
-
-  - intros.
+  - intros t H.
     destruct H as [k H].
-    assert (U := inverse_simulation).
-    specialize (U M (TM.start M) t k H).
-    apply U.
+    apply (inverse_simulation M (TM.start M) t k H).
 Qed.
-
 
 Theorem reduction :
   TM.HaltTM 1 ⪯ SBTM_HALT.
@@ -1682,8 +598,7 @@ Proof.
   exists (fun '(M, t) =>
     existT _ (M' M) (encode_config M (TM_facts.mk_mconfig (TM.start M) t))).
   move=> [M t]. split.
-  - cbn.
-  move=> /simulation [k Hk]. exists k.
-    by move: Hk => /steps_truncate.
-  - by move=> [k] /steps_truncate /inverse_simulation.
+  - move=> /simulation [k Hk]. exists k.
+    by move: Hk => /steps_truncate_tape_None.
+  - by move=> [k] /steps_truncate_tape_None /inverse_simulation.
 Qed.
